docs/03-formal-verification/easycrypt/ms/comparison/ComparisonPayloadSupportPublic.ec
@@ -1,0 +1,93 @@
+require import AllCore List Distr.
+require import Algebra QssmTypes FS SchnorrBranch TrueClause BitnessOne.
+require import ComparisonTypes ComparisonDigests ComparisonPayloadTypes ComparisonPayloadSeeds.
+require import ComparisonPayloadSupportTypes.
+
+(* Public-field obligation predicates and packaging lemmas. *)
+
+pred ms3c_ax_payload_public_fields_match (x : ms_public_input) (s : seed) =
+  forall (pr : ms3c_real_comparison_payload) (ps : ms3c_sim_comparison_payload),
+    ms3c_real_payload_on_support x pr =>
+    ms3c_sim_payload_on_support x s ps =>
+    ms3c_payload_pair_public_fields_match pr ps.
+
+pred ms3c_ax_payload_index_fields_match (x : ms_public_input) (s : seed) =
+  forall (pr : ms3c_real_comparison_payload) (ps : ms3c_sim_comparison_payload),
+    ms3c_real_payload_on_support x pr =>
+    ms3c_sim_payload_on_support x s ps =>
+    ms3c_payload_pair_index_fields_match pr ps.
+
+pred ms3c_ax_payload_ann_fields_match (x : ms_public_input) (s : seed) =
+  forall (pr : ms3c_real_comparison_payload) (ps : ms3c_sim_comparison_payload),
+    ms3c_real_payload_on_support x pr =>
+    ms3c_sim_payload_on_support x s ps =>
+    ms3c_payload_pair_ann_fields_match pr ps.
+
+pred ms3c_ax_payload_stmt_fields_match (x : ms_public_input) (s : seed) =
+  forall (pr : ms3c_real_comparison_payload) (ps : ms3c_sim_comparison_payload),
+    ms3c_real_payload_on_support x pr =>
+    ms3c_sim_payload_on_support x s ps =>
+    ms3c_payload_pair_stmt_fields_match pr ps.
+
+pred ms3c_ax_payload_result_fields_match (x : ms_public_input) (s : seed) =
+  forall (pr : ms3c_real_comparison_payload) (ps : ms3c_sim_comparison_payload),
+    ms3c_real_payload_on_support x pr =>
+    ms3c_sim_payload_on_support x s ps =>
+    ms3c_payload_pair_result_fields_match pr ps.
+
+lemma L_ms3c_ax_payload_public_fields_match_from_fragments
+  (x : ms_public_input) (s : seed) :
+  ms3c_ax_payload_index_fields_match x s =>
+  ms3c_ax_payload_ann_fields_match x s =>
+  ms3c_ax_payload_stmt_fields_match x s =>
+  ms3c_ax_payload_result_fields_match x s =>
+  ms3c_ax_payload_public_fields_match x s.
+proof.
+move=> Hix Hann Hstmt Hres.
+rewrite /ms3c_ax_payload_public_fields_match => pr ps Hpr Hps.
+move: (Hix pr ps Hpr Hps) (Hann pr ps Hpr Hps) (Hstmt pr ps Hpr Hps) (Hres pr ps Hpr Hps).
+move=> [Hi1 Hi2] [Ha1 Ha2] Hq [Hg Hp].
+rewrite /ms3c_payload_pair_public_fields_match.
+split; first exact Hi1.
+split; first exact Hi2.
+split; first exact Ha1.
+split; first exact Ha2.
+split; first exact Hq.
+split; first exact Hg.
+exact Hp.
+qed.
+
+pred ms3c_ax_payload_announcement_digests_preserved (x : ms_public_input) (s : seed) =
+  forall (pr : ms3c_real_comparison_payload) (ps : ms3c_sim_comparison_payload),
+    ms3c_real_payload_on_support x pr =>
+    ms3c_sim_payload_on_support x s ps =>
+    ms3c_clause_ann_digests_from_surface (ms3c_make_real_clause_surface pr) =
+    ms3c_clause_ann_digests_from_surface (ms3c_make_sim_clause_surface ps).
+
+pred ms3c_ax_payload_announcements_match_shape (x : ms_public_input) (s : seed) =
+  (forall (pr : ms3c_real_comparison_payload),
+    ms3c_real_payload_on_support x pr =>
+    ms3c_payload_ann_digest_list_shape_ok pr) /\
+  (forall (ps : ms3c_sim_comparison_payload),
+    ms3c_sim_payload_on_support x s ps =>
+    ms3c_payload_ann_digest_list_shape_ok ps).
+
+lemma L_ms3c_ax_payload_announcements_match_shape_total
+  (x : ms_public_input) (s : seed) :
+  ms3c_ax_payload_announcements_match_shape x s.
+proof.
+rewrite /ms3c_ax_payload_announcements_match_shape.
+split.
+  move=> pr _.
+  exact (L_ms3c_real_payload_ann_digest_list_shape_ok x pr).
+move=> ps _.
+exact (L_ms3c_sim_payload_ann_digest_list_shape_ok x s ps).
+qed.
+
+pred ms3c_ax_payload_challenge_share_consistency (x : ms_public_input) (s : seed) =
+  (forall (pr : ms3c_real_comparison_payload),
+    ms3c_real_payload_on_support x pr =>
+    ms3c_payload_programmed_challenge_matches_global pr) /\
+  (forall (ps : ms3c_sim_comparison_payload),
+    ms3c_sim_payload_on_support x s ps =>
+    ms3c_payload_programmed_challenge_matches_global ps).
